src/lowparse/LowParse.Spec.RtoLPair.fst
@@ -5,13 +5,14 @@ module Seq = FStar.Seq
 
 let nondep_then_rtol_kind 
   (k1: parser_kind { k1.parser_kind_subkind == Some ParserConsumesAll })
-  (n: nat)
+  (k2: parser_kind)
   : parser_kind
   = {
-      parser_kind_low = k1.parser_kind_low + n;
+      parser_kind_low = k1.parser_kind_low + k2.parser_kind_low;
       parser_kind_high = None;
       parser_kind_subkind = Some (ParserConsumesAll);
       parser_kind_metadata = None;
+      parser_kind_injective = k1.parser_kind_injective && k2.parser_kind_injective;
     }
 
 let nondep_then_rtol_bare
@@ -44,20 +45,23 @@ let nondep_then_rtol_bare_correct
   (#k1: parser_kind)
   (#t1: Type)
   (p1: parser k1 t1 { k1.parser_kind_subkind == Some ParserConsumesAll })
-  : Lemma (ensures parser_kind_prop (nondep_then_rtol_kind k1 k2.parser_kind_low) (nondep_then_rtol_bare
+  : Lemma (ensures parser_kind_prop (nondep_then_rtol_kind k1 k2) (nondep_then_rtol_bare
     p2 p1))
   = 
     Classical.forall_intro_2 (Seq.lemma_split # byte) ;
     parser_kind_prop_equiv k1 p1;
     parser_kind_prop_equiv k2 p2;
-    parser_kind_prop_equiv (nondep_then_rtol_kind k1 k2.parser_kind_low) (nondep_then_rtol_bare
+    parser_kind_prop_equiv (nondep_then_rtol_kind k1 k2) (nondep_then_rtol_bare
     p2 p1);
 
     let ps = nondep_then_rtol_bare p2 p1 in
     let f
       (b1 b2: bytes)
     : Lemma
-      (requires (injective_precond ps b1 b2))
+      (requires (
+        k1.parser_kind_injective /\ k2.parser_kind_injective /\
+        injective_precond ps b1 b2
+      ))
       (ensures (injective_postcond ps b1 b2))
     = 
       let (bl1, br1) = Seq.split b1 (Seq.length b1 - k2.parser_kind_low) in
@@ -67,7 +71,7 @@ let nondep_then_rtol_bare_correct
       assert (injective_postcond ps b1 b2)
     in
     Classical.forall_intro_2 (fun x -> Classical.move_requires (f x)) ; // add f to the SMT context
-    assert (injective (nondep_then_rtol_bare p2 p1));
+    assert ((nondep_then_rtol_kind k1 k2).parser_kind_injective ==> injective (nondep_then_rtol_bare p2 p1));
     assert (consumes_all (nondep_then_rtol_bare p2 p1));
     assert (parses_at_least (k1.parser_kind_low + k2.parser_kind_low) (nondep_then_rtol_bare p2 p1))
 
@@ -79,7 +83,7 @@ val parse_nondep_then_rtol
   (#k1: parser_kind)
   (#t1: Type)
   (p1: parser k1 t1 { k1.parser_kind_subkind == Some ParserConsumesAll })
-: Tot (parser (nondep_then_rtol_kind k1 k2.parser_kind_low) (t2 & t1))
+: Tot (parser (nondep_then_rtol_kind k1 k2) (t2 & t1))
 
 let parse_nondep_then_rtol
   (#k2: parser_kind)
@@ -88,7 +92,7 @@ let parse_nondep_then_rtol
   (#k1: parser_kind)
   (#t1: Type)
   (p1: parser k1 t1 { k1.parser_kind_subkind == Some ParserConsumesAll })
-  : Tot (parser (nondep_then_rtol_kind k1 k2.parser_kind_low) (t2 & t1)) =
+  : Tot (parser (nondep_then_rtol_kind k1 k2) (t2 & t1)) =
   nondep_then_rtol_bare_correct p2 p1;
   nondep_then_rtol_bare p2 p1
 
